---
title: Fermat 2004 Q24
author: Alan_Bui
date: 2022-12-07
categories: [Fermat]
tags: [functions, TO DO]
math: true
mermaid: true
---

---
## Problem Statement
The polynomial $f(x)$ satisfies the equation $f(x) - f(x - 2) = (2x - 1)^2 \;$ for all $x$. If $p$ and $q$ are the coefficients of $x^2$ and $x$, respectively, in $f(x)$, then $p + q$ equals 

[Problem Link](https://cemc.uwaterloo.ca/contests/past_contests/2004/2004FermatContest.pdf)

## Solution

$$f(x) - f(x - 2) = (2x - 1)^2 \;\; \forall x$$

$$x = \dfrac{1}{2}, \implies f(\dfrac{1}{2}) = f(\dfrac{-3}{2})$$

---